fix

Algorithm/Data/Classes/IndexedMinHeap.lean
@@ -190,7 +190,7 @@ def mk [DecidableEq α] (assocArray : C) (minHeap : C')
   else
     haveI : DecidableEq (WithIdx α ι) := by classical infer_instance
     have : size (MinHeap.tail minHeap) < size minHeap := by
-      simpa [h, size_eq_card_toMultiset, Multiset.card_erase_lt_of_mem, - MinHeap.head_def] using
+      simpa [h, size_eq_card_toMultiset, Multiset.card_erase_lt_of_mem] using
         Multiset.card_erase_lt_of_mem (MinHeap.head_mem_toMultiset _ _)
     mk assocArray (MinHeap.tail minHeap) fun i hi ↦ by
       simp only [← mem_toMultiset, MinHeap.toMultiset_tail, h, Bool.false_eq_true, ↓reduceDIte,
@@ -199,18 +199,15 @@ def mk [DecidableEq α] (assocArray : C) (minHeap : C')
       · exact mem_minHeap _ _
       · intro h''
         apply h'
-        simp [← h'']
+        simp [← h'', MinHeap.head_def]
 termination_by size minHeap
 
-@[simp]
+@[simp, nolint unusedHavesSuffices] -- false positive
 lemma mk_assocArray [DecidableEq α] (assocArray : C) (minHeap : C')
     (mem_minHeap : ∀ i : ι, (hi : assocArray[i] ≠ ⊤) → ⟨(assocArray[i]).untop hi, i⟩ ∈ minHeap) :
     (mk assocArray minHeap mem_minHeap).assocArray = assocArray := by
   induction minHeap, mem_minHeap using mk.induct
-  all_goals unfold mk; split_ifs
-  · rfl
-  · rfl
-  · assumption
+  all_goals unfold mk; simp [*]
 
 @[simp]
 lemma default_assocArray :
